MPL/ProofMode/Tactics/Basic.lean
@@ -5,7 +5,7 @@ open Lean Elab.Tactic Meta
 
 namespace MPL.ProofMode.Tactics
 
-def sstart (mvar : MVarId) : MetaM (MVarId × SGoal) := mvar.withContext do
+def mStart (mvar : MVarId) : MetaM (MVarId × SGoal) := mvar.withContext do
   -- check if already in proof mode
   let goal ← instantiateMVars <| ← mvar.getType
   if let some sGoal := parseSGoal? goal then
@@ -28,11 +28,11 @@ def sstart (mvar : MVarId) : MetaM (MVarId × SGoal) := mvar.withContext do
   let goal := { goal with target := ← instantiateMVars goal.target }
   pure (subgoal.mvarId!, goal)
 
-elab "sstart" : tactic => do
-  let (mvar, _) ← sstart (← getMainGoal)
+elab "mstart" : tactic => do
+  let (mvar, _) ← mStart (← getMainGoal)
   replaceMainGoal [mvar]
 
-elab "sstop" : tactic => do
+elab "mstop" : tactic => do
   -- parse goal
   let mvar ← getMainGoal
   mvar.withContext do
@@ -41,25 +41,3 @@ elab "sstop" : tactic => do
   -- check if already in proof mode
   let some sGoal := parseSGoal? goal | throwError "not in proof mode"
   mvar.setType sGoal.strip
-
-example (P Q : SPred [Nat, Bool]) : P ⊢ₛ Q := by
-  sstart
-  sstop
-  admit
-
-/-
--- theorem assumption [BI PROP] {p : Bool} {P P' A Q : PROP} [inst : FromAssumption p A Q]
---   [TCOr (Affine P') (Absorbing Q)] (h : P ⊣⊢ P' ∗ □?p A) : P ⊢ Q :=
---   h.1.trans <| (sep_mono_r inst.1).trans sep_elim_r
-
---def getFreshName : TSyntax ``binderIdent → CoreM (Name × Syntax)
---  | `(binderIdent| $name:ident) => pure (name.getId, name)
---  | stx => return (← mkFreshUserName `x, stx)
-
-def selectHyp (ty : Expr) : Hyps → MetaM Hyp
-  | .strue _ => failure
-  | .hyp h => do
-    let .true ← isDefEq ty h.p | failure
-    pure h
-  | .and _ lhs rhs => selectHyp ty rhs <|> selectHyp ty lhs
--/
