MPL/Utils/UnexpandRule.lean
@@ -1,0 +1,29 @@
+import Lean
+
+namespace MPL.Utils
+
+open Lean Macro Parser
+
+-- macro for adding unexpanders for function applications
+private def matchAlts' := leading_parser Term.matchAlts
+
+syntax "app_unexpand_rule" ident matchAlts' : command
+macro_rules
+  | `(app_unexpand_rule $f $[| $p => $s]*) => do
+    let f := f.getId
+    if f.isAnonymous then
+      throwUnsupported
+    let f ← match ← Macro.resolveGlobalName f with
+      | [(name, [])] => pure name
+      | _           => throwUnsupported
+
+    let (p : TSyntaxArray `term) := p
+    if p.any (· matches `(`($$_))) then
+      `(@[app_unexpander $(mkIdent f)]
+        def unexpand : Lean.PrettyPrinter.Unexpander
+          $[| $p => $s]*)
+    else
+      `(@[app_unexpander $(mkIdent f)]
+        def unexpand : Lean.PrettyPrinter.Unexpander
+          $[| $p => $s]*
+          | _ => throw ())
